examples/PolyApply/DemoPolyApply.v
@@ -1,0 +1,106 @@
+Require Import ExtLib.Core.RelDec. 
+Require Import ExtLib.Tactics.
+Require Import MirrorCore.Util.Compat.
+Require Import MirrorCore.Views.Ptrns.
+Require Import MirrorCore.Lambda.ExprCore.
+Require Import MirrorCore.Lambda.ExprD.
+Require Import MirrorCore.Lambda.RedAll.
+Require Import MirrorCore.Lambda.RewriteRelations.
+Require Import MirrorCore.Lambda.RewriteStrat.
+Require Import MirrorCore.Lambda.Red.
+Require Import MirrorCore.Lambda.Ptrns.
+Require Import MirrorCore.Lambda.Rewrite.HintDbs.
+Require Import MirrorCore.Reify.Reify.
+Require Import MirrorCore.RTac.IdtacK.
+Require Import MirrorCore.RTac.Intro.
+Require Import MirrorCore.RTac.Then.
+Require Import MirrorCore.RTac.RunOnGoals.
+Require Import MirrorCore.RTac.PApply.
+Require Import MirrorCore.MTypes.ModularTypes.
+Require Import MirrorCore.Polymorphic.
+Require Import MirrorCore.PLemma.
+
+Require Import McExamples.PolyRewrite.MSimple.
+Require Import McExamples.PolyRewrite.MSimpleReify.
+
+Existing Instance RType_typ.
+Existing Instance Expr.Expr_expr.
+Existing Instance Expr.ExprOk_expr.
+Existing Instance Typ2_Fun.
+Existing Instance Typ2Ok_Fun.
+
+Require Import MirrorCore.VariablesI.
+Require Import MirrorCore.Lambda.ExprVariables.
+
+Global Instance ExprVar_expr : ExprVar (expr typ func) := _.
+Global Instance ExprVarOk_expr : ExprVarOk ExprVar_expr := _.
+
+Global Instance ExprUVar_expr : ExprUVar (expr typ func) := _.
+Global Instance ExprUVarOk_expr : ExprUVarOk ExprUVar_expr := _.
+
+Definition subst : Type :=
+  FMapSubst.SUBST.raw (expr typ func).
+Global Instance SS : SubstI.Subst subst (expr typ func) :=
+  @FMapSubst.SUBST.Subst_subst _.
+Global Instance SU : SubstI.SubstUpdate subst (expr typ func) :=
+  @FMapSubst.SUBST.SubstUpdate_subst _ _ _ _.
+Check SubstI.SubstOk.
+Global Instance SO : @SubstI.SubstOk _ _ _ _ _ SS :=
+  @FMapSubst.SUBST.SubstOk_subst typ RType_typ (expr typ func) _.
+Global Instance SUO : @SubstI.SubstUpdateOk _ _ _ _ _ _ SU SO :=  @FMapSubst.SUBST.SubstUpdateOk_subst typ RType_typ (expr typ func) _ _.
+
+Definition fintro (e : expr typ func) : option (@OpenAs typ (expr typ func)) :=
+  match e with
+  | App (Inj (Ex t)) P => Some (AsEx t (fun x => beta (App P x)))
+  | App (Inj (All t)) P => Some (AsAl t (fun x => beta (App P x)))
+  | App (App (Inj Impl) P) Q => Some (AsHy P Q)
+  | _ => None
+  end.
+
+Definition INTRO := @INTRO typ (expr typ func) ExprVar_expr ExprUVar_expr fintro.
+
+
+Lemma forall_exists_eq {A : Type} : forall x : A, exists y, x = y.
+Proof.                                                  
+  intros.
+  exists x. reflexivity.
+Qed.
+
+Definition lem_forall_exists_eq : polymorphic typ 1 (Lemma.lemma typ (expr typ func) (expr typ func)) :=
+  Eval unfold Lemma.add_var, Lemma.add_prem , Lemma.vars , Lemma.concl , Lemma.premises in
+  <:: @forall_exists_eq ::>.
+
+Definition p_lem_forall_exists_eq : PolyLemma typ (expr typ func) (expr typ func) :=
+ {| p_n := 1;
+    p_lem := lem_forall_exists_eq;
+    p_tc := fun _ => true
+ |}.
+
+Print lem_forall_exists_eq.
+
+Let tyBNat := ModularTypes.tyBase0 tyNat.
+Let tyBBool := ModularTypes.tyBase0 tyBool.
+
+Definition fAnd a b : expr typ func := App (App (Inj MSimple.And) a) b.
+Definition fOr a b : expr typ func := App (App (Inj MSimple.And) a) b.
+Definition fAll t P : expr typ func := App (Inj (MSimple.All t)) (Abs t P).
+Definition fEx t P : expr typ func := App (Inj (MSimple.Ex t)) (Abs t P).
+Definition fEq t : expr typ func := (Inj (MSimple.Eq t)).
+Definition fImpl : expr typ func := (Inj MSimple.Impl).
+Definition mkEq t a b : expr typ func := App (App (fEq t) a) b.
+Definition fN n : expr typ func := Inj (MSimple.N n).
+
+Require Import MirrorCore.RTac.PApply.
+Require Import MirrorCore.Lambda.ExprUnify_simple.
+
+Definition PAPPLY (plem : PolyLemma typ (expr typ func) (expr typ func)) :=
+  PAPPLY 
+    (fun subst SS SU tus tvs n l r t s =>
+              @exprUnify subst typ func RType_typ RSym_func Typ2_Fun
+                         SS SU 10 tus tvs n l r t s) plem.
+
+Eval vm_compute in 
+    (THEN INTRO (runOnGoals (PAPPLY p_lem_forall_exists_eq))) 
+      (CTop nil nil) 
+      (TopSubst _ nil nil) 
+      (fAll tyBNat (fEx tyBNat (mkEq tyBNat (Var 1) (Var 0)))).
