examples/Tauto/ILogicFunc.v
@@ -1,0 +1,313 @@
+Require Import ExtLib.Core.RelDec.
+Require Import ExtLib.Data.Nat.
+Require Import ExtLib.Data.Bool.
+Require Import ExtLib.Data.String.
+Require Import ExtLib.Data.POption.
+Require Import ExtLib.Data.Map.FMapPositive.
+Require Import ExtLib.Data.SumN.
+Require Import ExtLib.Data.Positive.
+Require Import ExtLib.Tactics.
+Require Import ExtLib.Tactics.Consider.
+
+Require Import MirrorCore.TypesI.
+Require Import MirrorCore.syms.SymEnv.
+Require Import MirrorCore.Lambda.Expr.
+Require Import MirrorCore.Lambda.Ptrns.
+Require Import MirrorCore.SymI.
+Require Import MirrorCore.syms.SymSum.
+Require Import MirrorCore.Views.Ptrns.
+Require Import MirrorCore.Views.FuncView.
+Require Import MirrorCore.Reify.ReifyClass.
+
+Require Import McExamples.Tauto.ILogic.
+Require Import McExamples.Tauto.MSimpleTyp.
+
+Require Import Coq.Bool.Bool.
+
+
+Set Implicit Arguments.
+Set Strict Implicit.
+Set Maximal Implicit Insertion.
+
+Inductive ilfunc : Type :=
+  | ilf_entails (logic : typ)
+  | ilf_true (logic : typ)
+  | ilf_false (logic : typ)
+  | ilf_and (logic : typ)
+  | ilf_or (logic : typ)
+  | ilf_impl (logic : typ)
+  | ilf_exists (arg logic : typ)
+  | ilf_forall (arg logic : typ).
+
+Definition ilfunc_logic (x : ilfunc) : typ :=
+  match x with
+    | ilf_entails t => t
+    | ilf_true t => t
+    | ilf_false t => t
+    | ilf_and t => t
+    | ilf_or t => t
+    | ilf_impl t => t
+    | ilf_exists _ t => t
+    | ilf_forall _ t => t
+  end.
+
+Section ILogicFuncInst.
+  
+  Let tyArr : typ -> typ -> typ := @typ2 _ _ _ _.
+
+  Definition logic_ops := forall (t : typ),
+    poption (ILogicOps (typD t)).
+    
+  Definition logic_opsOk (l : logic_ops) : Prop :=
+    forall g, match l g return Prop with
+                | pSome T => @ILogic _ T
+                | pNone => True
+              end.
+
+  Variable gs : logic_ops.
+
+  Definition typeof_ilfunc (f : ilfunc) : option typ :=
+    match f with
+    | ilf_true t
+    | ilf_false t => match gs t with
+  		     | pSome _ => Some t
+		     | pNone => None
+  		     end
+    | ilf_entails t => match gs t with
+		       | pSome _ => Some (tyArr t (tyArr t tyProp))
+		       | pNone => None
+		       end
+    | ilf_and t
+    | ilf_or t
+    | ilf_impl t => match gs t with
+		    | pSome _ => Some (tyArr t (tyArr t t))
+		    | pNone => None
+		    end
+    | ilf_forall a t
+    | ilf_exists a t => match gs t with
+			| pSome _ => Some (tyArr (tyArr a t) t)
+			| pNone => None
+			end
+    end.
+  
+  Global Instance RelDec_ilfunc : RelDec (@eq ilfunc) :=
+    { rel_dec := fun a b =>
+	           match a, b with
+		   | ilf_entails t, ilf_entails t'
+		   | ilf_true t, ilf_true t'
+		   | ilf_false t, ilf_false t'
+		   | ilf_and t, ilf_and t'
+		   | ilf_or t, ilf_or t'
+		   | ilf_impl t, ilf_impl t' => t ?[eq] t'
+		   | ilf_forall a t, ilf_forall a' t'
+		   | ilf_exists a t, ilf_exists a' t' => (a ?[eq] a' && t ?[eq] t')%bool
+		   | _, _ => false
+	         end
+    }.
+
+  Global Instance RelDec_Correct_ilfunc : RelDec_Correct RelDec_ilfunc.
+  Proof.
+    constructor.
+    destruct x; destruct y; simpl;
+    try solve [ try rewrite Bool.andb_true_iff ;
+                repeat rewrite rel_dec_correct; intuition congruence ].
+  Qed.
+
+ Definition trueR {t : typ} {IL : ILogicOps (typD t)} := @ltrue (typD t) IL.
+ Definition falseR {t : typ} {IL : ILogicOps (typD t)} := @lfalse (typD t) IL.
+ Definition andR {t : typ} {IL : ILogicOps (typD t)} :=
+   castR id (RFun (typD t) (RFun (typD t) (typD t))) (@land (typD t) IL).
+ Definition orR {t : typ} {IL : ILogicOps (typD t)} :=
+   castR id (RFun (typD t) (RFun (typD t) (typD t))) (@lor (typD t) IL).
+ Definition implR {t : typ} {IL : ILogicOps (typD t)} :=
+   castR id (RFun (typD t) (RFun (typD t) (typD t))) (@limpl (typD t) IL).
+ Definition entailsR {t : typ} {IL : ILogicOps (typD t)} :=
+   castR id (RFun (typD t) (RFun (typD t) Prop)) (@lentails (typD t) IL).
+ Definition existsR {t u : typ} {IL : ILogicOps (typD t)} :=
+   castR id (RFun (RFun (typD u) (typD t)) (typD t)) (@lexists (typD t) IL (typD u)).
+ Definition forallR {t u : typ} {IL : ILogicOps (typD t)} :=
+   castR id (RFun (RFun (typD u) (typD t)) (typD t)) (@lforall (typD t) IL (typD u)).
+ 
+ Implicit Arguments trueR [[t] [IL]].
+ Implicit Arguments falseR [[t] [IL]].
+ Implicit Arguments andR [[t] [IL]]. 
+ Implicit Arguments orR [[t] [IL]].
+ Implicit Arguments implR [[t] [IL]].
+ 
+ Definition funcD (f : ilfunc) : match typeof_ilfunc f return Type with
+				     | Some t => typD t
+				     | None => unit
+				     end :=
+   match f as f
+         return match typeof_ilfunc f return Type with
+		| Some t => typD t
+		| None => unit
+		end
+   with
+   | ilf_true t => match gs t as x return (match match x with
+						 | pSome _ => Some t
+						 | pNone => None
+						 end with
+				           | Some t0 => typD t0
+					   | None => unit
+					   end) with
+		   | pSome t => @ltrue _ t
+		   | pNone => tt
+		   end
+   | ilf_false t =>
+     match gs t as x
+           return (match match x with
+			 | pSome _ => Some t
+			 | pNone => None
+			 end with
+		   | Some t0 => typD t0
+		   | None => unit
+		   end) with
+     | pSome t => lfalse
+     | pNone => tt
+     end
+   | ilf_entails t =>
+     match gs t as x
+           return (match match x with
+			 | pSome _ => Some (tyArr t (tyArr t tyProp))
+			 | pNone => None
+			 end with
+		   | Some t0 => typD t0
+		   | None => unit
+		   end) with
+     | pSome t => entailsR
+     | pNone => tt
+     end
+   | ilf_and t =>
+     match gs t as x
+           return (match match x with
+			 | pSome _ => Some (tyArr t (tyArr t t))
+			 | pNone => None
+			 end with
+		   | Some t0 => typD t0
+		   | None => unit
+		   end) with
+     | pSome t => andR
+     | pNone => tt
+     end
+   | ilf_impl t =>
+     match gs t as x
+           return (match match x with
+			 | pSome _ => Some (tyArr t (tyArr t t))
+			 | pNone => None
+			 end with
+		   | Some t0 => typD t0
+		   | None => unit
+		   end) with
+     | pSome t => implR
+     | pNone => tt
+     end
+   | ilf_or t =>
+     match gs t as x
+           return (match match x with
+			 | pSome _ => Some (tyArr t (tyArr t t))
+			 | pNone => None
+			 end with
+		   | Some t0 => typD t0
+		   | None => unit
+		   end) with
+     | pSome t => orR
+     | pNone => tt
+     end
+   | ilf_exists a t =>
+     match gs t as x return (match match x with
+				   | pSome _ => Some (tyArr (tyArr a t) t)
+				   | pNone => None
+				   end with
+			     | Some t0 => typD t0
+			     | None => unit
+			     end) with
+     | pSome t0 => existsR
+     | pNone => tt
+     end
+   | ilf_forall a t =>
+     match gs t as x return (match match x with
+				   | pSome _ => Some (tyArr (tyArr a t) t)
+				   | pNone => None
+				   end with
+			     | Some t0 => typD t0
+			     | None => unit
+			     end) with
+     | pSome t0 => forallR
+     | pNone => tt
+     end
+   end.
+ 
+End ILogicFuncInst.
+
+
+Section MakeILogic.
+  Variable t u : typ.
+
+  Definition fTrue := ilf_true t.
+  Definition fFalse := ilf_false t.
+  Definition fAnd := ilf_and t.
+  Definition fOr := ilf_or t.
+  Definition fImpl := ilf_impl t.
+  Definition fEntails := ilf_entails t.
+  Definition fExists := ilf_exists t u.
+  Definition fForall := ilf_forall t u.
+
+  Definition mkEntails (P Q : expr typ ilfunc) := App (App (Inj fEntails) P) Q.
+  Definition mkTrue : expr typ ilfunc := Inj fTrue.
+  Definition mkFalse : expr typ ilfunc := Inj fFalse.
+  Definition mkAnd (P Q : expr typ ilfunc) := App (App (Inj fAnd) P) Q.
+  Definition mkOr (P Q : expr typ ilfunc) := App (App (Inj fOr) P) Q.
+  Definition mkImpl (P Q : expr typ ilfunc) := App (App (Inj fImpl) P) Q.
+  Definition mkExists (f : expr typ ilfunc) := App (Inj fExists) (Abs t f).
+  Definition mkForall (f : expr typ ilfunc) := App (Inj fForall) (Abs t f).
+
+End MakeILogic.
+
+Require Import MirrorCore.VariablesI.
+Require Import MirrorCore.Lambda.ExprVariables.
+Require Import MirrorCore.Subst.FMapSubst.
+
+Definition gs : logic_ops :=
+  fun t => 
+    match t with
+    | ModularTypes.tyProp => pSome _
+    | _ => pNone
+    end.
+
+Global Instance RSym_ilfunc : SymI.RSym ilfunc :=
+  { typeof_sym := typeof_ilfunc gs
+    ; sym_eqb := fun a b => Some (rel_dec a b)
+    ; symD := funcD gs
+  }.
+
+Global Instance RSymOk_ilfunc : SymI.RSymOk RSym_ilfunc.
+Proof.
+  constructor.
+  intros. unfold sym_eqb; simpl.
+  consider (a ?[ eq ] b); auto.
+Qed.
+
+
+Global Instance Expr_expr : ExprI.Expr _ (expr typ ilfunc) := @Expr_expr typ ilfunc _ _ _.
+
+Global Instance Expr_ok : @ExprI.ExprOk typ RType_typ (expr typ ilfunc) Expr_expr := 
+  @ExprOk_expr typ ilfunc _ _ _ _ _ _.
+
+Global Instance ExprVar_expr : ExprVar (expr typ ilfunc) := _.
+
+Global Instance ExprVarOk_expr : ExprVarOk ExprVar_expr := _.
+
+Global Instance ExprUVar_expr : ExprUVar (expr typ ilfunc) := _.
+Global Instance ExprUVarOk_expr : ExprUVarOk ExprUVar_expr := _.
+
+Definition subst : Type :=
+  FMapSubst.SUBST.raw (expr typ ilfunc).
+Global Instance SS : SubstI.Subst subst (expr typ ilfunc) :=
+  @FMapSubst.SUBST.Subst_subst _.
+Global Instance SU : SubstI.SubstUpdate subst (expr typ ilfunc) :=
+  @FMapSubst.SUBST.SubstUpdate_subst _ _ _ _.
+Check SubstI.SubstOk.
+Global Instance SO : @SubstI.SubstOk _ _ _ _ _ SS :=
+  @FMapSubst.SUBST.SubstOk_subst typ RType_typ (expr typ ilfunc) _.
+Global Instance SUO : @SubstI.SubstUpdateOk _ _ _ _ _ _ SU SO :=  @FMapSubst.SUBST.SubstUpdateOk_subst typ RType_typ (expr typ ilfunc) _ _.
