examples/Tauto/ILogicReify.v
@@ -1,0 +1,110 @@
+Require Import Coq.Lists.List.
+Require Import MirrorCore.Reify.Reify.
+Require Import MirrorCore.MTypes.ModularTypes.
+Require Import MirrorCore.Lambda.ExprCore.
+Require Import McExamples.Tauto.MSimpleTyp.
+Require Import McExamples.Tauto.ILogic.
+Require Import McExamples.Tauto.ILogicFunc.
+
+Require Import MirrorCore.PLemma.
+Require Import MirrorCore.RTac.PApply.
+Require Import MirrorCore.Lambda.ExprUnify_simple.
+
+(** Declare patterns **)
+Reify Declare Patterns patterns_simple_typ : typ.
+Reify Declare Patterns patterns_ilfunc : (expr typ ilfunc).
+
+Reify Declare Syntax reify_simple_typ :=
+  CPatterns patterns_simple_typ.
+
+Axiom otherFunc : BinNums.positive -> expr typ ilfunc.
+
+Reify Declare Typed Table table_terms : BinNums.positive => typ.
+
+(** Declare syntax **)
+Reify Declare Syntax reify_ilfunc :=
+  CFix
+    (CFirst (CPatterns patterns_ilfunc ::
+             CApp (CRec 0) (CRec 0) (@ExprCore.App typ ilfunc) ::
+             CAbs (CCall reify_simple_typ) (CRec 0) (@ExprCore.Abs typ ilfunc) ::
+             CVar (@ExprCore.Var typ ilfunc) ::
+             CMap otherFunc (CTypedTable (CCall reify_simple_typ) table_terms)
+             :: nil)).
+
+Local Notation "x @ y" := (@RApp x y) (only parsing, at level 30).
+Local Notation "'!!' x" := (@RExact _ x) (only parsing, at level 25).
+Local Notation "'?' n" := (@RGet n RIgnore) (only parsing, at level 25).
+Local Notation "'?!' n" := (@RGet n RConst) (only parsing, at level 25).
+Local Notation "'#'" := RIgnore (only parsing, at level 0).
+
+Reify Pattern patterns_simple_typ += (!! nat)  => (tyNat).
+Reify Pattern patterns_simple_typ += (!! bool) => (tyBool).
+Reify Pattern patterns_simple_typ += (!! Prop) => (tyProp).
+Reify Pattern patterns_simple_typ += (@RImpl (@RGet 0 RIgnore) (@RGet 1 RIgnore)) => (fun (a b : function (CCall reify_simple_typ)) => tyArr a b).
+
+Reify Pattern patterns_ilfunc += (!! @ILogic.ltrue @ ?0 @ #) =>
+  (fun (x : function (CCall reify_simple_typ)) => mkTrue x).
+Reify Pattern patterns_ilfunc += (!! @ILogic.lfalse @ ?0 @ #) =>
+  (fun (x : function (CCall reify_simple_typ)) => mkFalse x).
+Reify Pattern patterns_ilfunc += (!! @ILogic.land @ ?0 @ #) =>
+  (fun (x : function (CCall reify_simple_typ)) => Inj (typ := typ) (fAnd x)).
+Reify Pattern patterns_ilfunc += (!! @ILogic.lor @ ?0 @ #) =>
+  (fun (x : function (CCall reify_simple_typ)) => Inj (typ := typ) (fOr x)).
+Reify Pattern patterns_ilfunc += (!! @ILogic.limpl @ ?0 @ #) =>
+  (fun (x : function (CCall reify_simple_typ)) => Inj (typ := typ) (fImpl x)).
+Reify Pattern patterns_ilfunc += (!! @ILogic.lentails @ ?0 @ #) =>
+  (fun (x : function (CCall reify_simple_typ)) => Inj (typ := typ) (fEntails x)).
+Reify Pattern patterns_ilfunc += (!! @ILogic.lexists @ ?0 @ # @ ?1) => (fun (x y : function (CCall reify_simple_typ)) => Inj (typ := typ) (fExists y x)).
+Reify Pattern patterns_ilfunc += (!! @ILogic.lforall @ ?0 @ # @ ?1) => (fun (x y : function (CCall reify_simple_typ)) => Inj (typ := typ) (fForall y x)).
+
+Instance Reify_expr_ilfunc : Reify (expr typ ilfunc) :=
+{ reify_scheme := CCall reify_ilfunc }.
+
+Instance Reify_simple_type : Reify typ :=
+{ reify_scheme := CCall reify_simple_typ }.
+
+Ltac reify_typ trm :=
+  let k e :=
+      refine e
+  in
+  reify_expr reify_simple_typ k [[ True ]] [[ trm ]].
+
+Ltac reify trm :=
+  let k e :=
+      refine e
+  in
+  reify_expr reify_ilfunc k [[ True ]] [[ trm ]].
+
+Ltac reify_ilfunc trm k :=
+  reify_expr reify_ilfunc k [[ True ]] [[ trm ]].
+
+
+Definition test_typ : typ.
+  reify_typ (nat -> nat).
+Defined.
+Print test_typ.
+
+Definition test_typ_2 : typ.
+  reify_typ ((nat -> nat) -> nat -> (nat -> nat -> nat -> nat)).
+Defined.
+Print test_typ_2.
+
+Definition test_1 : expr typ ilfunc.
+  reify (@ltrue Prop _).
+Defined.
+Print test_1.
+
+Definition test_2 : expr typ ilfunc.
+  reify (@lfalse Prop _).                      
+Defined.
+Print test_2.
+
+Definition test_3 : expr typ ilfunc.
+  reify (@land Prop _ (@ltrue Prop _) (@lfalse Prop _)).
+Defined.
+Print test_3.
+
+Definition test_4 (P : nat -> Prop) : expr typ ilfunc.
+  reify (@lexists Prop _ nat P).
+Defined.
+Print test_4.
