examples/Tauto/Tauto.v
@@ -1,0 +1,73 @@
+Require Import Coq.Lists.List.
+Require Import MirrorCore.MTypes.ModularTypes.
+Require Import MirrorCore.Lambda.ExprCore.
+Require Import McExamples.Tauto.MSimpleTyp.
+Require Import McExamples.Tauto.ILogic.
+Require Import McExamples.Tauto.ILogicFunc.
+Require Import McExamples.Tauto.ILogicReify.
+
+Require Import MirrorCore.PLemma.
+Require Import MirrorCore.RTac.PApply.
+Require Import MirrorCore.Lemma.
+Require Import MirrorCore.Polymorphic.
+Require Import MirrorCore.Lambda.ExprUnify_simple.
+Require Import MirrorCore.RTac.RTac.
+
+Definition tc (t : typ) :=
+  match t with
+    | ModularTypes.tyProp => true
+    | _ => true
+  end.
+
+Definition r_trueR : PolyLemma typ (expr typ ilfunc) (expr typ ilfunc) :=
+  {| p_n := 1;
+     p_lem := fun t => 
+               {| vars := t :: nil;
+                  premises := nil;
+                  concl := App (App (Inj (fEntails t)) (Var 0)) (mkTrue t) |};
+     p_tc := tc
+  |}.
+
+Definition r_falseL : PolyLemma typ (expr typ ilfunc) (expr typ ilfunc) :=
+  {| p_n := 1;
+     p_lem := fun t => 
+               {| vars := t :: nil;
+                  premises := nil;
+                  concl := App (App (Inj (fEntails t)) (mkFalse t)) (Var 0) |};
+     p_tc := tc
+  |}.
+
+Definition r_andR : PolyLemma typ (expr typ ilfunc) (expr typ ilfunc) :=
+  {| p_n := 1;
+     p_lem := fun t => 
+               {| vars := t :: nil;
+                  premises := App (App (Inj (fEntails t)) (Var 0)) (Var 2)
+                                  :: App (App (Inj (fEntails t)) (Var 0)) (Var 1) :: nil;
+                  concl := App (App (Inj (fEntails t)) (Var 0))
+                               (App (App (Inj (fAnd t)) (Var 2)) (Var 1)) |};
+     p_tc := tc
+  |}.
+
+Definition PAPPLY (plem : PolyLemma typ (expr typ ilfunc) (expr typ ilfunc)) :=
+  PAPPLY 
+    (fun subst SS SU tus tvs n l r t s =>
+              @exprUnify subst typ ilfunc RType_typ RSym_ilfunc Typ2_Fun
+                         SS SU 10 tus tvs n l r t s) plem.
+
+
+Definition TAUTO : rtac typ (expr typ ilfunc) :=
+  REC 10
+      (fun r =>
+         (FIRST
+            (PAPPLY r_trueR ::
+             PAPPLY r_falseL :: 
+             THEN (PAPPLY r_andR) (runOnGoals r) :: nil))) FAIL.
+
+Goal True.
+pose (PApply.get_lemma r_trueR
+           (mkEntails tyProp (mkTrue tyProp) (mkTrue tyProp))).
+compute in o.
+(* Gregory, I'm pretty sure this should be evaluate to Some *)
+
+apply I.
+Qed.
