theories/PLemma.v
@@ -1,0 +1,15 @@
+Require Import MirrorCore.Lemma.
+Require Import MirrorCore.Polymorphic.
+
+Section PolyLemma.
+  Context {typ expr conclusion : Type}.
+
+  Record PolyLemma := {
+    p_n : nat;                    
+    p_lem : polymorphic typ p_n (lemma typ expr conclusion);
+    p_tc : polymorphic typ p_n bool
+  }.
+
+End PolyLemma.
+
+Arguments PolyLemma : clear implicits.
